matching-logic/src/Theories/Bool_ProofSystem.v
@@ -20,7 +20,7 @@ Context
   Proof.
     intro HΓ.
     apply useBasicReasoning.
-    apply BasicProofSystemLemmas.hypothesis.
+    apply hypothesis.
     { destruct ax; wf_auto2. }
     {
       apply elem_of_weaken with (X := theory_of_NamedAxioms named_axioms).
